src/study/Nemonuri.Study.CSharpSyntaxRewriter2.Modifier2/Nemonuri.StratifiedNodes.Indexes.fst
@@ -1,0 +1,14 @@
+module Nemonuri.StratifiedNodes.Indexes
+
+module L = FStar.List.Tot
+module N = Nemonuri.StratifiedNodes.Nodes
+module C = Nemonuri.StratifiedNodes.Children
+module Common = Nemonuri.StratifiedNodes.Common
+
+//--- theory members ---
+let to_indexes #t (ancestors:C.ancestor_list t)
+  : Pure (list nat) (requires True) (ensures fun r -> true)
+  =
+  ()
+
+//---|
